Incremental API for ML-KEM

libcrux-ml-kem/c/libcrux_mlkem768_portable.c
@@ -4,11 +4,11 @@
  * SPDX-License-Identifier: MIT or Apache-2.0
  *
  * This code was generated with the following revisions:
- * Charon: 30cab88265206f4fa849736e704983e39a404d96
- * Eurydice: b8ea420ccde8db516ced5db9c097d77fa558fb94
- * Karamel: 97a06e07e7e423df192c40d5a88bf6c85fd4d278
+ * Charon: a8f2211d1b95e0462a96382023b164a4116c7ca4
+ * Eurydice: 60f543ddc60a777138070968daaf7620ec48170d
+ * Karamel: 1d81d757d5d9e16dd6463ccc72324e587c707959
  * F*: b0961063393215ca65927f017720cb365a193833-dirty
- * Libcrux: 15b22d1beea1cc7052b8a68b653b012241724664
+ * Libcrux: e2291b6e918559a4712b2a553f49ec92fdba1e42
  */
 
 #include "libcrux_mlkem768_portable.h"
@@ -113,16 +113,15 @@ generics
 - CPA_PRIVATE_KEY_SIZE= 1152
 - PRIVATE_KEY_SIZE= 2400
 - PUBLIC_KEY_SIZE= 1184
-- RANKED_BYTES_PER_RING_ELEMENT= 1152
 - ETA1= 2
 - ETA1_RANDOMNESS_SIZE= 128
 */
-static libcrux_ml_kem_mlkem768_MlKem768KeyPair generate_keypair_c6(
+static libcrux_ml_kem_mlkem768_MlKem768KeyPair generate_keypair_ce(
     uint8_t randomness[64U]) {
   /* Passing arrays by value in Rust generates a copy in C */
   uint8_t copy_of_randomness[64U];
   memcpy(copy_of_randomness, randomness, (size_t)64U * sizeof(uint8_t));
-  return libcrux_ml_kem_ind_cca_generate_keypair_f8(copy_of_randomness);
+  return libcrux_ml_kem_ind_cca_generate_keypair_15(copy_of_randomness);
 }
 
 /**
@@ -133,7 +132,7 @@ libcrux_ml_kem_mlkem768_portable_generate_key_pair(uint8_t randomness[64U]) {
   /* Passing arrays by value in Rust generates a copy in C */
   uint8_t copy_of_randomness[64U];
   memcpy(copy_of_randomness, randomness, (size_t)64U * sizeof(uint8_t));
-  return generate_keypair_c6(copy_of_randomness);
+  return generate_keypair_ce(copy_of_randomness);
 }
 
 /**
@@ -198,11 +197,10 @@ A monomorphic instance of
 libcrux_ml_kem.ind_cca.instantiations.portable.validate_public_key with const
 generics
 - K= 3
-- RANKED_BYTES_PER_RING_ELEMENT= 1152
 - PUBLIC_KEY_SIZE= 1184
 */
-static KRML_MUSTINLINE bool validate_public_key_31(uint8_t *public_key) {
-  return libcrux_ml_kem_ind_cca_validate_public_key_6c(public_key);
+static KRML_MUSTINLINE bool validate_public_key_41(uint8_t *public_key) {
+  return libcrux_ml_kem_ind_cca_validate_public_key_89(public_key);
 }
 
 /**
@@ -212,5 +210,5 @@ static KRML_MUSTINLINE bool validate_public_key_31(uint8_t *public_key) {
 */
 bool libcrux_ml_kem_mlkem768_portable_validate_public_key(
     libcrux_ml_kem_types_MlKemPublicKey_30 *public_key) {
-  return validate_public_key_31(public_key->value);
+  return validate_public_key_41(public_key->value);
 }
