libcrux-ml-kem/src/mlkem.rs
@@ -1,0 +1,830 @@
+#![cfg(feature = "incremental")]
+
+//! Top level entry points for ML-KEM
+//!
+//! For now this is only used for the incremental API.
+
+// This should be replaced with a nicer proc macro later.
+
+macro_rules! impl_incr_key_size {
+    () => {
+        use crate::ind_cca::incremental::multiplexing;
+
+        use self::incremental::types::{self, Error};
+        pub use self::incremental::types::{PublicKey1, PublicKey2};
+
+        use super::*;
+        use ind_cca::incremental;
+
+        /// Ciphertext 1
+        pub type Ciphertext1 = types::Ciphertext1<C1_SIZE>;
+
+        /// Ciphertext 2
+        pub type Ciphertext2 = types::Ciphertext2<C2_SIZE>;
+
+        /// Get the size of the first public key in bytes.
+        pub const fn pk1_len() -> usize {
+            PublicKey1::len()
+        }
+
+        /// Get the size of the second public key in bytes.
+        pub const fn pk2_len() -> usize {
+            RANKED_BYTES_PER_RING_ELEMENT
+        }
+
+        /// The size of a compressed key pair in bytes.
+        pub const COMPRESSED_KEYPAIR_LEN: usize = SECRET_KEY_SIZE;
+
+        /// The size of the key pair in bytes.
+        pub const fn key_pair_len() -> usize {
+            // Because const generics are too limited, we compute it here from scratch.
+
+            // PK1
+            pk1_len()
+            // PK2
+            + pk2_len()
+            // SK
+            + RANK * 16 * 32 + 32
+            // Matrix
+            + RANK * RANK * 16 * 32
+        }
+
+
+        /// The size of the compressed key pair in bytes.
+        pub const fn key_pair_compressed_len() -> usize {
+            COMPRESSED_KEYPAIR_LEN
+        }
+
+        /// The size of the encaps state in bytes.
+        pub const fn encaps_state_len() -> usize {
+            // Because const generics are too limited, we compute it here from scratch.
+
+            // r_as_ntt
+            RANK * 16 * 32
+            // error2
+            + 16 * 32
+            // randomness
+            + 32
+        }
+
+        /// The size of the shared secret.
+        pub const fn shared_secret_size() -> usize {
+            SHARED_SECRET_SIZE
+        }
+
+        /// Functions in this module require an allocator to use [`Box`].
+        ///
+        /// Instead of serializing keys and state, the functions in this module return
+        /// the platform dependent keys and state types for immediate use.
+        #[cfg(feature = "alloc")]
+        pub mod alloc {
+            use super::*;
+            use super::incremental::types::alloc::{State, Keys};
+            use ::alloc::boxed::Box;
+
+            /// Generate a new key pair for incremental encapsulation.
+            pub fn generate_key_pair(randomness: [u8; KEY_GENERATION_SEED_SIZE]) -> Box<dyn Keys> {
+                multiplexing::alloc::generate_keypair::<
+                    RANK,
+                    CPA_PKE_SECRET_KEY_SIZE,
+                    SECRET_KEY_SIZE,
+                    CPA_PKE_PUBLIC_KEY_SIZE,
+                    RANKED_BYTES_PER_RING_ELEMENT,
+                    ETA1,
+                    ETA1_RANDOMNESS_SIZE,
+                >(randomness)
+            }
+
+            /// Encapsulate the first part of the ciphertext.
+            pub fn encapsulate1(
+                public_key_part: &PublicKey1,
+                randomness: [u8; SHARED_SECRET_SIZE],
+            ) -> (Ciphertext1, Box<dyn State>, [u8; SHARED_SECRET_SIZE]) {
+                multiplexing::alloc::encapsulate1::<
+                    RANK,
+                    CPA_PKE_CIPHERTEXT_SIZE,
+                    C1_SIZE,
+                    VECTOR_U_COMPRESSION_FACTOR,
+                    C1_BLOCK_SIZE,
+                    ETA1,
+                    ETA1_RANDOMNESS_SIZE,
+                    ETA2,
+                    ETA2_RANDOMNESS_SIZE,
+                >(public_key_part, randomness)
+            }
+
+            /// Encapsulate the second part of the ciphertext.
+            ///
+            /// The second part of the public key is passed in as byte slice.
+            /// [`Error::InvalidInputLength`] is returned if `public_key_part` is too
+            /// short.
+            pub fn encapsulate2(state: &dyn State, public_key_part: &[u8]) -> Result<Ciphertext2, Error> {
+                multiplexing::alloc::encapsulate2::<RANK, RANKED_BYTES_PER_RING_ELEMENT, C2_SIZE, VECTOR_V_COMPRESSION_FACTOR>(
+                    state,
+                    public_key_part,
+                )
+            }
+
+            /// Decapsulate incremental ciphertexts.
+            pub fn decapsulate(
+                private_key: &dyn Keys,
+                ciphertext1: &Ciphertext1,
+                ciphertext2: &Ciphertext2,
+            ) -> MlKemSharedSecret {
+                multiplexing::alloc::decapsulate::<
+                    RANK,
+                    SECRET_KEY_SIZE,
+                    CPA_PKE_SECRET_KEY_SIZE,
+                    CPA_PKE_PUBLIC_KEY_SIZE,
+                    CPA_PKE_CIPHERTEXT_SIZE,
+                    T_AS_NTT_ENCODED_SIZE,
+                    C1_SIZE,
+                    C2_SIZE,
+                    VECTOR_U_COMPRESSION_FACTOR,
+                    VECTOR_V_COMPRESSION_FACTOR,
+                    C1_BLOCK_SIZE,
+                    ETA1,
+                    ETA1_RANDOMNESS_SIZE,
+                    ETA2,
+                    ETA2_RANDOMNESS_SIZE,
+                    IMPLICIT_REJECTION_HASH_INPUT_SIZE,
+                >(private_key, ciphertext1, ciphertext2)
+            }
+        }
+
+        /// An encoded, incremental key pair.
+        pub struct KeyPairBytes {
+            value: [u8; key_pair_len()]
+        }
+
+        #[cfg(all(not(eurydice), feature = "rand"))]
+        use ::rand::{CryptoRng, RngCore};
+
+        impl KeyPairBytes {
+            /// Generate a new key pair.
+            /// This uses unpacked keys and does not compress the keys.
+            pub fn from_seed(randomness: [u8; KEY_GENERATION_SEED_SIZE]) -> Self {
+                let mut out = Self {
+                    value: [0u8; key_pair_len()]
+                };
+                generate_key_pair(randomness, &mut out.value).unwrap();
+                out
+            }
+
+            /// Generate a new key pair.
+            /// This uses unpacked keys and does not compress the keys.
+            #[cfg(all(not(eurydice), feature = "rand"))]
+            pub fn generate(rng: &mut (impl RngCore + CryptoRng)) -> Self {
+                let mut randomness = [0u8; KEY_GENERATION_SEED_SIZE];
+                rng.fill_bytes(&mut randomness);
+                let mut out = Self {
+                    value: [0u8; key_pair_len()]
+                };
+                generate_key_pair(randomness, &mut out.value).unwrap();
+                out
+            }
+
+            /// Get the raw bytes.
+            pub fn to_bytes(self) -> [u8; key_pair_len()] {
+                self.value
+            }
+
+            /// Get the PK1 bytes from the serialized key pair bytes
+            pub fn pk1(&self) -> &[u8; pk1_len()] {
+                // The unwrap here is ok because that's exactly what we take
+                // and we know that `self.value` is long enough.
+                <&[u8; pk1_len()]>::try_from(&self.value[0..pk1_len()]).unwrap()
+            }
+
+            /// Get the PK2 bytes from the serialized key pair bytes
+            pub fn pk2(&self) -> &[u8; pk2_len()] {
+                // The unwrap here is ok because that's exactly what we take
+                // and we know that `self.value` is long enough.
+                <&[u8; pk2_len()]>::try_from(&self.value[pk1_len()..pk1_len() + pk2_len()]).unwrap()
+            }
+        }
+
+        impl AsRef<[u8]> for KeyPairBytes {
+            fn as_ref(&self) -> &[u8] {
+                &self.value
+            }
+        }
+
+        /// Generate a key pair and write it into `key_pair`.
+        /// This uses unpacked keys and does not compress the keys.
+        ///
+        /// `key_pair.len()` must be of size `key_pair_len()`.
+        /// The function returns an error if this is not the case.
+        pub fn generate_key_pair(randomness: [u8; KEY_GENERATION_SEED_SIZE], key_pair: &mut [u8]) -> Result<(), Error> {
+            multiplexing::generate_keypair::<
+                RANK,
+                RANKED_BYTES_PER_RING_ELEMENT,
+                CPA_PKE_SECRET_KEY_SIZE,
+                SECRET_KEY_SIZE,
+                CPA_PKE_PUBLIC_KEY_SIZE,
+                RANKED_BYTES_PER_RING_ELEMENT,
+                ETA1,
+                ETA1_RANDOMNESS_SIZE,
+            >(randomness, key_pair)
+        }
+        /// An encoded, compressed, incremental key pair.
+        ///
+        /// Layout: dk | (t | ⍴) | H(ek) | z
+        pub struct KeyPairCompressedBytes {
+            value: [u8; key_pair_compressed_len()]
+        }
+
+        impl KeyPairCompressedBytes {
+            /// Generate a new key pair.
+            /// This uses unpacked keys and does not compress the keys.
+            pub fn from_seed(randomness: [u8; KEY_GENERATION_SEED_SIZE]) -> Self {
+                let mut out = Self {
+                    value: [0u8; key_pair_compressed_len()]
+                };
+                generate_key_pair_compressed(randomness, &mut out.value);
+                out
+            }
+
+            /// Generate a new key pair.
+            /// This uses unpacked keys and does not compress the keys.
+            #[cfg(all(not(eurydice), feature = "rand"))]
+            pub fn generate(rng: &mut (impl RngCore + CryptoRng)) -> Self {
+                let mut randomness = [0u8; KEY_GENERATION_SEED_SIZE];
+                rng.fill_bytes(&mut randomness);
+                let mut out = Self {
+                    value: [0u8; key_pair_compressed_len()]
+                };
+                generate_key_pair_compressed(randomness, &mut out.value);
+                out
+            }
+
+            /// Get the raw bytes.
+            pub fn to_bytes(self) -> [u8; key_pair_compressed_len()] {
+                self.value
+            }
+
+            /// Get the PK1 bytes from the serialized key pair bytes
+            pub fn pk1(&self) -> &[u8; pk1_len()] {
+                // The unwrap here is ok because that's exactly what we take
+                // and we know that `self.value` is long enough.
+                const START: usize = 2 *  RANKED_BYTES_PER_RING_ELEMENT;
+                <&[u8; pk1_len()]>::try_from(&self.value[START..START + pk1_len()]).unwrap()
+            }
+
+            /// Get the PK2 bytes from the serialized key pair bytes
+            pub fn pk2(&self) -> &[u8; pk2_len()] {
+                // The unwrap here is ok because that's exactly what we take
+                // and we know that `self.value` is long enough.
+                const START: usize = RANKED_BYTES_PER_RING_ELEMENT;
+                <&[u8; pk2_len()]>::try_from(&self.value[START..START + pk2_len()]).unwrap()
+            }
+
+            /// Get the serialized private for decapsulation.
+            pub fn sk(&self) -> &[u8; SECRET_KEY_SIZE] {
+                &self.value
+            }
+        }
+
+        impl AsRef<[u8]> for KeyPairCompressedBytes {
+            fn as_ref(&self) -> &[u8] {
+                &self.value
+            }
+        }
+
+        /// Generate a key pair and write it into `key_pair`.
+        /// This compresses the keys.
+        pub fn generate_key_pair_compressed(randomness: [u8; KEY_GENERATION_SEED_SIZE], key_pair: &mut [u8; COMPRESSED_KEYPAIR_LEN]) {
+            multiplexing::generate_keypair_compressed::<
+                RANK,
+                RANKED_BYTES_PER_RING_ELEMENT,
+                CPA_PKE_SECRET_KEY_SIZE,
+                SECRET_KEY_SIZE,
+                CPA_PKE_PUBLIC_KEY_SIZE,
+                RANKED_BYTES_PER_RING_ELEMENT,
+                ETA1,
+                ETA1_RANDOMNESS_SIZE,
+                COMPRESSED_KEYPAIR_LEN,
+            >(randomness, key_pair)
+        }
+
+        /// Get the PK1 bytes from the serialized key pair bytes
+        pub fn pk1(
+            keypair: &[u8; key_pair_len()],
+        ) -> &[u8] {
+            &keypair[0..pk1_len()]
+        }
+
+        /// Get the PK2 bytes from the serialized key pair bytes
+        pub fn pk2(
+            keypair: &[u8; key_pair_len()],
+        ) -> &[u8] {
+            &keypair[pk1_len()..pk1_len() + pk2_len()]
+        }
+
+        /// Validate that the two parts `pk1` and `pk2` are consistent.
+        pub fn validate_pk(
+            pk1: &PublicKey1,
+            pk2: &[u8],
+        ) -> Result<(), Error> {
+            multiplexing::validate_pk::<RANK,  CPA_PKE_PUBLIC_KEY_SIZE>(pk1, pk2)
+        }
+
+        /// Validate that the two parts `pk1` and `pk2` are consistent.
+        pub fn validate_pk_bytes(
+            pk1: &[u8],
+            pk2: &[u8],
+        ) -> Result<(), Error> {
+            multiplexing::validate_pk_bytes::<RANK,  CPA_PKE_PUBLIC_KEY_SIZE>(pk1, pk2)
+        }
+
+        /// Encapsulate the first part of the ciphertext.
+        ///
+        /// Returns an [`Error`] if the provided input or output don't have
+        /// the appropriate sizes.
+        pub fn encapsulate1(
+            pk1: &[u8],
+            randomness: [u8; SHARED_SECRET_SIZE],
+            state: &mut [u8],
+            shared_secret: &mut [u8],
+        ) -> Result<Ciphertext1, Error> {
+            let public_key_part = PublicKey1::try_from(&pk1 as &[u8])?;
+
+            multiplexing::encapsulate1::<
+                RANK,
+                CPA_PKE_CIPHERTEXT_SIZE,
+                C1_SIZE,
+                VECTOR_U_COMPRESSION_FACTOR,
+                C1_BLOCK_SIZE,
+                ETA1,
+                ETA1_RANDOMNESS_SIZE,
+                ETA2,
+                ETA2_RANDOMNESS_SIZE,
+            >(&public_key_part, randomness, state, shared_secret)
+        }
+
+        /// Encapsulate the first part of the ciphertext.
+        ///
+        /// Returns an [`Error`] if the provided input or output don't have
+        /// the appropriate sizes.
+        #[cfg(feature = "rand")]
+        pub mod rand {
+            use super::*;
+
+            /// Encapsulate the first part of the ciphertext.
+            ///
+            /// Returns an [`Error`] if the provided input or output don't have
+            /// the appropriate sizes.
+            pub fn encapsulate1(
+                pk1: &[u8],
+                rng: &mut (impl RngCore + CryptoRng),
+                state: &mut [u8],
+                shared_secret: &mut [u8],
+            ) -> Result<Ciphertext1, Error> {
+                let public_key_part = PublicKey1::try_from(&pk1 as &[u8])?;
+                let mut randomness = [0u8; SHARED_SECRET_SIZE];
+                rng.try_fill_bytes(&mut randomness).map_err(|_| Error::InsufficientRandomness)?;
+
+                multiplexing::encapsulate1::<
+                    RANK,
+                    CPA_PKE_CIPHERTEXT_SIZE,
+                    C1_SIZE,
+                    VECTOR_U_COMPRESSION_FACTOR,
+                    C1_BLOCK_SIZE,
+                    ETA1,
+                    ETA1_RANDOMNESS_SIZE,
+                    ETA2,
+                    ETA2_RANDOMNESS_SIZE,
+                >(&public_key_part, randomness, state, shared_secret)
+            }
+        }
+
+        /// Encapsulate the second part of the ciphertext.
+        ///
+        /// The second part of the public key is passed in as byte slice.
+        /// [`Error::InvalidInputLength`] is returned if `public_key_part` is too
+        /// short.
+        pub fn encapsulate2(state: &[u8; encaps_state_len()], public_key_part: &[u8; pk2_len()]) -> Ciphertext2 {
+            multiplexing::encapsulate2::<RANK, RANKED_BYTES_PER_RING_ELEMENT, C2_SIZE, VECTOR_V_COMPRESSION_FACTOR, {encaps_state_len()}>(state, public_key_part)
+        }
+
+        /// Decapsulate incremental ciphertexts.
+        pub fn decapsulate_incremental_key(
+            private_key: &[u8],
+            ciphertext1: &Ciphertext1,
+            ciphertext2: &Ciphertext2,
+        ) -> Result<MlKemSharedSecret, Error> {
+            multiplexing::decapsulate::<
+                RANK,
+                RANKED_BYTES_PER_RING_ELEMENT,
+                SECRET_KEY_SIZE,
+                CPA_PKE_SECRET_KEY_SIZE,
+                CPA_PKE_PUBLIC_KEY_SIZE,
+                CPA_PKE_CIPHERTEXT_SIZE,
+                T_AS_NTT_ENCODED_SIZE,
+                C1_SIZE,
+                C2_SIZE,
+                VECTOR_U_COMPRESSION_FACTOR,
+                VECTOR_V_COMPRESSION_FACTOR,
+                C1_BLOCK_SIZE,
+                ETA1,
+                ETA1_RANDOMNESS_SIZE,
+                ETA2,
+                ETA2_RANDOMNESS_SIZE,
+                IMPLICIT_REJECTION_HASH_INPUT_SIZE,
+            >(private_key, ciphertext1, ciphertext2)
+        }
+
+        /// Decapsulate incremental ciphertexts.
+        pub fn decapsulate_compressed_key(
+            private_key: &[u8; SECRET_KEY_SIZE],
+            ciphertext1: &Ciphertext1,
+            ciphertext2: &Ciphertext2,
+        ) -> MlKemSharedSecret {
+            multiplexing::decapsulate_compressed::<
+                RANK,
+                RANKED_BYTES_PER_RING_ELEMENT,
+                SECRET_KEY_SIZE,
+                CPA_PKE_SECRET_KEY_SIZE,
+                CPA_PKE_PUBLIC_KEY_SIZE,
+                CPA_PKE_CIPHERTEXT_SIZE,
+                T_AS_NTT_ENCODED_SIZE,
+                C1_SIZE,
+                C2_SIZE,
+                VECTOR_U_COMPRESSION_FACTOR,
+                VECTOR_V_COMPRESSION_FACTOR,
+                C1_BLOCK_SIZE,
+                ETA1,
+                ETA1_RANDOMNESS_SIZE,
+                ETA2,
+                ETA2_RANDOMNESS_SIZE,
+                IMPLICIT_REJECTION_HASH_INPUT_SIZE,
+            >(private_key, ciphertext1, ciphertext2)
+        }
+    };
+}
+pub(crate) use impl_incr_key_size;
+
+macro_rules! impl_incr_platform {
+    ($vector:path, $hash:path $(, $unsafe:ident)? $(, #[$meta:meta])*) => {
+        /// Downcast [`Keys`] to a platform dependent [`MlKemKeyPairUnpacked`].
+        ///
+        /// **PANICS** is the cast fails
+        #[cfg(feature = "alloc")]
+        pub(super) fn as_keypair<const K: usize>(
+            k: &dyn core::any::Any,
+        ) -> &MlKemKeyPairUnpacked<K, $vector> {
+            k.downcast_ref().unwrap()
+        }
+
+        /// Downcast [`State`] to a  platform dependent [`EncapsState`].
+        ///
+        /// **PANICS** is the cast fails
+        #[cfg(feature = "alloc")]
+        pub(super) fn as_state<const K: usize>(s: &dyn core::any::Any) -> &EncapsState<K, $vector> {
+            s.downcast_ref().unwrap()
+        }
+
+        $(#[$meta])*
+        pub(crate) $($unsafe)? fn generate_keypair<
+            const K: usize,
+            const CPA_PRIVATE_KEY_SIZE: usize,
+            const PRIVATE_KEY_SIZE: usize,
+            const PUBLIC_KEY_SIZE: usize,
+            const BYTES_PER_RING_ELEMENT: usize,
+            const ETA1: usize,
+            const ETA1_RANDOMNESS_SIZE: usize,
+        >(
+            randomness: [u8; KEY_GENERATION_SEED_SIZE],
+        ) -> MlKemKeyPairUnpacked<K, $vector> {
+            super::generate_keypair::<
+                K,
+                CPA_PRIVATE_KEY_SIZE,
+                PRIVATE_KEY_SIZE,
+                PUBLIC_KEY_SIZE,
+                ETA1,
+                ETA1_RANDOMNESS_SIZE,
+                $vector,
+                $hash,
+            >(randomness)
+        }
+
+        $(#[$meta])*
+        pub(crate) $($unsafe)? fn generate_keypair_serialized<
+            const K: usize,
+            const PK2_LEN: usize,
+            const CPA_PRIVATE_KEY_SIZE: usize,
+            const PRIVATE_KEY_SIZE: usize,
+            const PUBLIC_KEY_SIZE: usize,
+            const BYTES_PER_RING_ELEMENT: usize,
+            const ETA1: usize,
+            const ETA1_RANDOMNESS_SIZE: usize,
+        >(
+            randomness: [u8; KEY_GENERATION_SEED_SIZE],
+            key_pair: &mut [u8],
+        ) -> Result<(), Error> {
+            if key_pair.len() < KeyPair::<K, PK2_LEN, $vector>::num_bytes() {
+                return Err(Error::InvalidOutputLength);
+            }
+
+            super::generate_keypair_serialized::<
+                K,
+                PK2_LEN,
+                CPA_PRIVATE_KEY_SIZE,
+                PRIVATE_KEY_SIZE,
+                PUBLIC_KEY_SIZE,
+                ETA1,
+                ETA1_RANDOMNESS_SIZE,
+                $vector,
+                $hash,
+            >(randomness, key_pair)
+        }
+
+        $(#[$meta])*
+        pub(crate) $($unsafe)? fn generate_keypair_compressed<
+            const K: usize,
+            const PK2_LEN: usize,
+            const CPA_PRIVATE_KEY_SIZE: usize,
+            const PRIVATE_KEY_SIZE: usize,
+            const PUBLIC_KEY_SIZE: usize,
+            const BYTES_PER_RING_ELEMENT: usize,
+            const ETA1: usize,
+            const ETA1_RANDOMNESS_SIZE: usize,
+            const COMPRESSED_KEYPAIR_LEN: usize,
+        >(
+            randomness: [u8; KEY_GENERATION_SEED_SIZE],
+            key_pair: &mut [u8; COMPRESSED_KEYPAIR_LEN],
+        ) {
+            super::generate_keypair_compressed::<
+                K,
+                PK2_LEN,
+                CPA_PRIVATE_KEY_SIZE,
+                PRIVATE_KEY_SIZE,
+                PUBLIC_KEY_SIZE,
+                ETA1,
+                ETA1_RANDOMNESS_SIZE,
+                COMPRESSED_KEYPAIR_LEN,
+                $vector,
+                $hash,
+            >(randomness, key_pair)
+        }
+
+        $(#[$meta])*
+        pub(crate) $($unsafe)? fn validate_pk<const K: usize, const PK_LEN: usize>(
+            pk1: &PublicKey1,
+            pk2: &[u8],
+        ) -> Result<(), Error> {
+            super::validate_pk::<K, PK_LEN, $hash, $vector>(pk1, pk2)
+        }
+
+        $(#[$meta])*
+        pub(crate) $($unsafe)? fn validate_pk_bytes<const K: usize, const PK_LEN: usize>(
+            pk1: &[u8],
+            pk2: &[u8],
+        ) -> Result<(), Error> {
+            super::validate_pk_bytes::<K, PK_LEN, $hash, $vector>(pk1, pk2)
+        }
+
+        $(#[$meta])*
+        pub(crate) $($unsafe)? fn encapsulate1<
+            const K: usize,
+            const CIPHERTEXT_SIZE: usize,
+            const C1_SIZE: usize,
+            const VECTOR_U_COMPRESSION_FACTOR: usize,
+            const VECTOR_U_BLOCK_LEN: usize,
+            const ETA1: usize,
+            const ETA1_RANDOMNESS_SIZE: usize,
+            const ETA2: usize,
+            const ETA2_RANDOMNESS_SIZE: usize,
+        >(
+            public_key_part: &PublicKey1,
+            randomness: [u8; SHARED_SECRET_SIZE],
+        ) -> (
+            Ciphertext1<C1_SIZE>,
+            EncapsState<K, $vector>,
+            [u8; SHARED_SECRET_SIZE],
+        ) {
+            super::encapsulate1::<
+                K,
+                CIPHERTEXT_SIZE,
+                C1_SIZE,
+                VECTOR_U_COMPRESSION_FACTOR,
+                VECTOR_U_BLOCK_LEN,
+                ETA1,
+                ETA1_RANDOMNESS_SIZE,
+                ETA2,
+                ETA2_RANDOMNESS_SIZE,
+                $vector,
+                $hash,
+            >(public_key_part, randomness)
+        }
+
+        $(#[$meta])*
+        pub(crate) $($unsafe)? fn encapsulate1_serialized<
+            const K: usize,
+            const CIPHERTEXT_SIZE: usize,
+            const C1_SIZE: usize,
+            const VECTOR_U_COMPRESSION_FACTOR: usize,
+            const VECTOR_U_BLOCK_LEN: usize,
+            const ETA1: usize,
+            const ETA1_RANDOMNESS_SIZE: usize,
+            const ETA2: usize,
+            const ETA2_RANDOMNESS_SIZE: usize,
+        >(
+            public_key_part: &PublicKey1,
+            randomness: [u8; SHARED_SECRET_SIZE],
+            state: &mut [u8],
+            shared_secret: &mut [u8],
+        ) -> Result<Ciphertext1<C1_SIZE>, Error> {
+            super::encapsulate1_serialized::<
+                K,
+                CIPHERTEXT_SIZE,
+                C1_SIZE,
+                VECTOR_U_COMPRESSION_FACTOR,
+                VECTOR_U_BLOCK_LEN,
+                ETA1,
+                ETA1_RANDOMNESS_SIZE,
+                ETA2,
+                ETA2_RANDOMNESS_SIZE,
+                $vector,
+                $hash,
+            >(public_key_part, randomness, state, shared_secret)
+        }
+
+        $(#[$meta])*
+        pub(crate) $($unsafe)? fn encapsulate2<
+            const K: usize,
+            const PK2_LEN: usize,
+            const C2_SIZE: usize,
+            const VECTOR_V_COMPRESSION_FACTOR: usize,
+        >(
+            state: &EncapsState<K, $vector>,
+            public_key_part: &PublicKey2<PK2_LEN>,
+        ) -> Ciphertext2<C2_SIZE> {
+            super::encapsulate2::<K, PK2_LEN, C2_SIZE, VECTOR_V_COMPRESSION_FACTOR, $vector>(
+                state,
+                public_key_part,
+            )
+        }
+
+        $(#[$meta])*
+        pub(crate) $($unsafe)? fn encapsulate2_serialized<
+            const K: usize,
+            const PK2_LEN: usize,
+            const C2_SIZE: usize,
+            const VECTOR_V_COMPRESSION_FACTOR: usize,
+            const STATE_LEN: usize,
+        >(
+            state: &[u8; STATE_LEN],
+            public_key_part: &PublicKey2<PK2_LEN>,
+        ) -> Ciphertext2<C2_SIZE> {
+            super::encapsulate2_serialized::<
+                K,
+                PK2_LEN,
+                C2_SIZE,
+                VECTOR_V_COMPRESSION_FACTOR,
+                STATE_LEN,
+                $vector,
+            >(state, public_key_part)
+        }
+
+        $(#[$meta])*
+        pub(crate) $($unsafe)? fn decapsulate<
+            const K: usize,
+            const SECRET_KEY_SIZE: usize,
+            const CPA_SECRET_KEY_SIZE: usize,
+            const PUBLIC_KEY_SIZE: usize,
+            const CIPHERTEXT_SIZE: usize,
+            const T_AS_NTT_ENCODED_SIZE: usize,
+            const C1_SIZE: usize,
+            const C2_SIZE: usize,
+            const VECTOR_U_COMPRESSION_FACTOR: usize,
+            const VECTOR_V_COMPRESSION_FACTOR: usize,
+            const C1_BLOCK_SIZE: usize,
+            const ETA1: usize,
+            const ETA1_RANDOMNESS_SIZE: usize,
+            const ETA2: usize,
+            const ETA2_RANDOMNESS_SIZE: usize,
+            const IMPLICIT_REJECTION_HASH_INPUT_SIZE: usize,
+        >(
+            private_key: &MlKemKeyPairUnpacked<K, $vector>,
+            ciphertext1: &Ciphertext1<C1_SIZE>,
+            ciphertext2: &Ciphertext2<C2_SIZE>,
+        ) -> MlKemSharedSecret {
+            super::decapsulate::<
+                K,
+                SECRET_KEY_SIZE,
+                CPA_SECRET_KEY_SIZE,
+                PUBLIC_KEY_SIZE,
+                CIPHERTEXT_SIZE,
+                T_AS_NTT_ENCODED_SIZE,
+                C1_SIZE,
+                C2_SIZE,
+                VECTOR_U_COMPRESSION_FACTOR,
+                VECTOR_V_COMPRESSION_FACTOR,
+                C1_BLOCK_SIZE,
+                ETA1,
+                ETA1_RANDOMNESS_SIZE,
+                ETA2,
+                ETA2_RANDOMNESS_SIZE,
+                IMPLICIT_REJECTION_HASH_INPUT_SIZE,
+                $vector,
+                $hash,
+            >(private_key, ciphertext1, ciphertext2)
+        }
+
+        $(#[$meta])*
+        pub(crate) $($unsafe)? fn decapsulate_incremental_key<
+            const K: usize,
+            const PK2_LEN: usize,
+            const SECRET_KEY_SIZE: usize,
+            const CPA_SECRET_KEY_SIZE: usize,
+            const PUBLIC_KEY_SIZE: usize,
+            const CIPHERTEXT_SIZE: usize,
+            const T_AS_NTT_ENCODED_SIZE: usize,
+            const C1_SIZE: usize,
+            const C2_SIZE: usize,
+            const VECTOR_U_COMPRESSION_FACTOR: usize,
+            const VECTOR_V_COMPRESSION_FACTOR: usize,
+            const C1_BLOCK_SIZE: usize,
+            const ETA1: usize,
+            const ETA1_RANDOMNESS_SIZE: usize,
+            const ETA2: usize,
+            const ETA2_RANDOMNESS_SIZE: usize,
+            const IMPLICIT_REJECTION_HASH_INPUT_SIZE: usize,
+        >(
+            private_key: &[u8],
+            ciphertext1: &Ciphertext1<C1_SIZE>,
+            ciphertext2: &Ciphertext2<C2_SIZE>,
+        ) -> Result<MlKemSharedSecret, Error> {
+            super::decapsulate_incremental_key::<
+                K,
+                PK2_LEN,
+                SECRET_KEY_SIZE,
+                CPA_SECRET_KEY_SIZE,
+                PUBLIC_KEY_SIZE,
+                CIPHERTEXT_SIZE,
+                T_AS_NTT_ENCODED_SIZE,
+                C1_SIZE,
+                C2_SIZE,
+                VECTOR_U_COMPRESSION_FACTOR,
+                VECTOR_V_COMPRESSION_FACTOR,
+                C1_BLOCK_SIZE,
+                ETA1,
+                ETA1_RANDOMNESS_SIZE,
+                ETA2,
+                ETA2_RANDOMNESS_SIZE,
+                IMPLICIT_REJECTION_HASH_INPUT_SIZE,
+                $vector,
+                $hash,
+            >(private_key, ciphertext1, ciphertext2)
+        }
+
+        $(#[$meta])*
+        pub(crate) $($unsafe)? fn decapsulate_compressed_key<
+            const K: usize,
+            const PK2_LEN: usize,
+            const SECRET_KEY_SIZE: usize,
+            const CPA_SECRET_KEY_SIZE: usize,
+            const PUBLIC_KEY_SIZE: usize,
+            const CIPHERTEXT_SIZE: usize,
+            const T_AS_NTT_ENCODED_SIZE: usize,
+            const C1_SIZE: usize,
+            const C2_SIZE: usize,
+            const VECTOR_U_COMPRESSION_FACTOR: usize,
+            const VECTOR_V_COMPRESSION_FACTOR: usize,
+            const C1_BLOCK_SIZE: usize,
+            const ETA1: usize,
+            const ETA1_RANDOMNESS_SIZE: usize,
+            const ETA2: usize,
+            const ETA2_RANDOMNESS_SIZE: usize,
+            const IMPLICIT_REJECTION_HASH_INPUT_SIZE: usize,
+        >(
+            private_key: &[u8; SECRET_KEY_SIZE],
+            ciphertext1: &Ciphertext1<C1_SIZE>,
+            ciphertext2: &Ciphertext2<C2_SIZE>,
+        ) -> MlKemSharedSecret {
+            super::decapsulate_compressed_key::<
+                K,
+                PK2_LEN,
+                SECRET_KEY_SIZE,
+                CPA_SECRET_KEY_SIZE,
+                PUBLIC_KEY_SIZE,
+                CIPHERTEXT_SIZE,
+                T_AS_NTT_ENCODED_SIZE,
+                C1_SIZE,
+                C2_SIZE,
+                VECTOR_U_COMPRESSION_FACTOR,
+                VECTOR_V_COMPRESSION_FACTOR,
+                C1_BLOCK_SIZE,
+                ETA1,
+                ETA1_RANDOMNESS_SIZE,
+                ETA2,
+                ETA2_RANDOMNESS_SIZE,
+                IMPLICIT_REJECTION_HASH_INPUT_SIZE,
+                $vector,
+                $hash,
+            >(private_key, ciphertext1, ciphertext2)
+        }
+    };
+}
+pub(crate) use impl_incr_platform;
