libcrux-intrinsics/proofs/fstar/extraction/Libcrux_intrinsics.Arm64_extract.fst
@@ -1,5 +1,5 @@
 module Libcrux_intrinsics.Arm64_extract
-#set-options "--fuel 0 --ifuel 1 --z3rlimit 80"
+#set-options "--fuel 0 --ifuel 1 --z3rlimit 15"
 open Core
 open FStar.Mul
 
@@ -18,6 +18,17 @@ val e_vst1q_s16': out: t_Slice i16 -> v: u8
   -> Prims.Pure (t_Slice i16) Prims.l_True (fun _ -> Prims.l_True)
 
 let e_vst1q_s16 = e_vst1q_s16'
+
+assume
+val e_vst1q_bytes': out: t_Slice u8 -> v: u8
+  -> Prims.Pure (t_Slice u8) Prims.l_True (fun _ -> Prims.l_True)
+
+let e_vst1q_bytes = e_vst1q_bytes'
+
+assume
+val e_vld1q_bytes': bytes: t_Slice u8 -> Prims.Pure u8 Prims.l_True (fun _ -> Prims.l_True)
+
+let e_vld1q_bytes = e_vld1q_bytes'
 
 assume
 val e_vld1q_s16': array: t_Slice i16 -> Prims.Pure u8 Prims.l_True (fun _ -> Prims.l_True)
