libcrux-ml-kem/proofs/fstar/extraction/Libcrux_ml_kem.Constants.fst
@@ -1,0 +1,7 @@
+module Libcrux_ml_kem.Constants
+#set-options "--fuel 0 --ifuel 1 --z3rlimit 80"
+open Core
+open FStar.Mul
+
+let ranked_bytes_per_ring_element (rank: usize) =
+  (rank *! v_BITS_PER_RING_ELEMENT <: usize) /! mk_usize 8
